WIP multiple updates

theories/multiple_updates.v
@@ -11,56 +11,68 @@ Section std_updates.
 
   Context {Σ:gFunctors}
     {ceriseg:ceriseG Σ}
+    {Cname : CmptNameG}
     {stsg : STSG Addr region_type Σ}
-    {heapg : heapGS Σ}.
+    {heapg : heapGS Σ}
+    `{MP: MachineParameters}.
 
   Notation STS := (leibnizO (STS_states * STS_rels)).
   Notation STS_STD := (leibnizO (STS_std_states Addr region_type)).
-  Notation WORLD := (prodO STS_STD STS).
+  Notation CVIEW := (prodO STS_STD STS).
+  Notation WORLD := (gmapO CmptName CVIEW).
+  Implicit Types WC : CVIEW.
   Implicit Types W : WORLD.
+  Implicit Types C : CmptName.
 
-  Fixpoint std_update_multiple W l ρ :=
+  Fixpoint std_update_multiple WC l ρ :=
     match l with
-    | [] => W
-    | a :: l => std_update (std_update_multiple W l ρ) a ρ
+    | [] => WC
+    | a :: l => std_update (std_update_multiple WC l ρ) a ρ
     end.
 
-   Definition std_update_temp_multiple W l := std_update_multiple W l Temporary.
+  Definition std_update_multiple_C W C l ρ :=
+    match W !! C with
+    | Some WC => <[C := std_update_multiple WC l ρ]> W
+    | None => W
+    end.
 
-   Lemma std_update_multiple_loc_sta W l ρ :
-     (std_update_multiple W l ρ).2.1 = W.2.1.
+   Definition std_update_temp_multiple WC l := std_update_multiple WC l Temporary.
+   Definition std_update_temp_multiple_C W C l := std_update_multiple_C W C l Temporary.
+
+   Lemma std_update_multiple_loc_sta WC l ρ :
+     (std_update_multiple WC l ρ).2.1 = WC.2.1.
    Proof.
      induction l; auto.
    Qed.
 
-   Lemma std_update_multiple_loc_rel W l ρ :
-     (std_update_multiple W l ρ).2.2 = W.2.2.
+   Lemma std_update_multiple_loc_rel WC l ρ :
+     (std_update_multiple WC l ρ).2.2 = WC.2.2.
    Proof.
      induction l; auto.
    Qed.
 
-   Lemma std_update_multiple_loc W l ρ :
-     (std_update_multiple W l ρ).2 = W.2.
+   Lemma std_update_multiple_loc WC l ρ :
+     (std_update_multiple WC l ρ).2 = WC.2.
    Proof.
      induction l; auto.
    Qed.
 
-   Lemma std_update_multiple_proj_eq W Wloc l ρ :
-     ((std_update_multiple W l ρ).1, Wloc) = std_update_multiple (W.1,Wloc) l ρ.
+   Lemma std_update_multiple_proj_eq WC Wloc l ρ :
+     ((std_update_multiple WC l ρ).1, Wloc) = std_update_multiple (WC.1,Wloc) l ρ.
    Proof.
-     destruct W as [Wsta Wloc']. simpl. induction l; auto.
+     destruct WC as [Wsta Wloc']. simpl. induction l; auto.
      simpl. rewrite -IHl. auto.
    Qed.
 
-   Lemma std_update_multiple_std_sta_eq W Wloc l ρ :
-     (std_update_multiple W l ρ).1 = (std_update_multiple (W.1, Wloc) l ρ).1.
+   Lemma std_update_multiple_std_sta_eq WC Wloc l ρ :
+     (std_update_multiple WC l ρ).1 = (std_update_multiple (WC.1, Wloc) l ρ).1.
    Proof.
-     destruct W as [Wsta Wloc']. simpl. induction l; auto.
+     destruct WC as [Wsta Wloc']. simpl. induction l; auto.
      simpl. rewrite -IHl. auto.
    Qed.
 
-   Lemma std_update_multiple_swap_head W l a1 a2 ρ :
-     std_update_multiple W (a1 :: a2 :: l) ρ = std_update_multiple W (a2 :: a1 :: l) ρ.
+   Lemma std_update_multiple_swap_head WC l a1 a2 ρ :
+     std_update_multiple WC (a1 :: a2 :: l) ρ = std_update_multiple WC (a2 :: a1 :: l) ρ.
    Proof.
      induction l.
      - simpl. destruct (decide (a1 = a2)); subst.
@@ -72,8 +84,8 @@ Section std_updates.
        repeat rewrite (insert_commute _ a1 a2) ; auto.
    Qed.
 
-   Lemma std_update_multiple_swap W l1 a l2 ρ :
-     std_update_multiple W (l1 ++ a :: l2) ρ = std_update_multiple W (a :: l1 ++ l2) ρ.
+   Lemma std_update_multiple_swap WC l1 a l2 ρ :
+     std_update_multiple WC (l1 ++ a :: l2) ρ = std_update_multiple WC (a :: l1 ++ l2) ρ.
    Proof.
      induction l1; auto.
      rewrite app_comm_cons std_update_multiple_swap_head /=.
@@ -81,22 +93,35 @@ Section std_updates.
    Qed.
 
 
-   Lemma std_update_multiple_permutation W l1 l2 ρ :
+   Lemma std_update_multiple_permutation WC l1 l2 ρ :
      l1 ≡ₚ l2 →
-     std_update_multiple W l1 ρ = std_update_multiple W l2 ρ.
+     std_update_multiple WC l1 ρ = std_update_multiple WC l2 ρ.
    Proof.
      intros Hperm.
      induction Hperm using Permutation_ind.
      - done.
      - simpl. rewrite IHHperm. done.
-     - apply (std_update_multiple_swap_head W l y x).
+     - apply (std_update_multiple_swap_head WC l y x).
      - by rewrite IHHperm1 IHHperm2.
    Qed.
 
-   Global Instance std_update_multiple_Permutation W ρ :
-     Proper (Permutation ==> eq) (λ l, std_update_multiple W l ρ).
+   Lemma std_update_multiple_permutation_C W C l1 l2 ρ :
+     l1 ≡ₚ l2 →
+     std_update_multiple_C W C l1 ρ = std_update_multiple_C W C l2 ρ.
+   Proof.
+     intros Hperm.
+     rewrite /std_update_multiple_C.
+     destruct (W!!C); last done.
+     erewrite std_update_multiple_permutation; eauto.
+   Qed.
+
+   Global Instance std_update_multiple_Permutation WC ρ :
+     Proper (Permutation ==> eq) (λ l, std_update_multiple WC l ρ).
    Proof. intros y1 y2 Hperm. simpl. by apply std_update_multiple_permutation. Defined.
 
+   Global Instance std_update_multiple_Permutation_C W C ρ :
+     Proper (Permutation ==> eq) (λ l, std_update_multiple_C W C l ρ).
+   Proof. intros y1 y2 Hperm. by apply std_update_multiple_permutation_C. Defined.
 
    Lemma remove_dups_swap_head {A : Type} `{EqDecision A} (a1 a2 : A) (l : list A) :
      remove_dups (a1 :: a2 :: l) ≡ₚ remove_dups (a2 :: a1 :: l).
@@ -146,9 +171,9 @@ Section std_updates.
    (* --------------------------------------------------------------------------------------------------------- *)
 
    (* If an element is not in the update list, the state lookup is the same *)
-   Lemma std_sta_update_multiple_lookup_same_i W l ρ i :
-     i ∉ l -> (std (std_update_multiple W l ρ)) !! i =
-             (std W) !! i.
+   Lemma std_sta_update_multiple_lookup_same_i WC l ρ i :
+     i ∉ l -> (std (std_update_multiple WC l ρ)) !! i =
+             (std WC) !! i.
    Proof.
      intros Hnin.
      induction l; auto.
@@ -159,8 +184,8 @@ Section std_updates.
    (* ------------------------------------------------------------ *)
 
    (* If an element is in the update list, the state lookup corresponds to the update value *)
-   Lemma std_sta_update_multiple_lookup_in_i W l ρ i :
-     i ∈ l -> (std (std_update_multiple W l ρ)) !! i = Some ρ.
+   Lemma std_sta_update_multiple_lookup_in_i WC l ρ i :
+     i ∈ l -> (std (std_update_multiple WC l ρ)) !! i = Some ρ.
    Proof.
      intros Hnin.
      induction l; auto; first inversion Hnin.
@@ -173,8 +198,8 @@ Section std_updates.
    (* ------------------------------------------------------------ *)
 
    (* if W at a is_Some, the the updated W at a is_Some *)
-   Lemma std_sta_update_multiple_is_Some W l ρ i :
-     is_Some (std W !! i) -> is_Some (std (std_update_multiple W l ρ) !! i).
+   Lemma std_sta_update_multiple_is_Some WC l ρ i :
+     is_Some (std WC !! i) -> is_Some (std (std_update_multiple WC l ρ) !! i).
    Proof.
      intros Hsome.
      destruct (decide (i ∈ l)).
@@ -185,17 +210,17 @@ Section std_updates.
    (* ------------------------------------------------------------ *)
 
    (* domains *)
-   Lemma std_update_multiple_not_in_sta_i W l ρ i :
-     i ∉ l → i ∈ dom (std W) ↔
-               i ∈ dom (std (std_update_multiple W l ρ)).
+   Lemma std_update_multiple_not_in_sta_i WC l ρ i :
+     i ∉ l → i ∈ dom (std WC) ↔
+               i ∈ dom (std (std_update_multiple WC l ρ)).
    Proof.
      intros Hnin. induction l; auto.
      apply not_elem_of_cons in Hnin as [Hneq Hnin].
      rewrite /= dom_insert. set_solver.
    Qed.
-   Lemma std_update_multiple_in_sta_i W (l: list Addr) ρ i :
-     Forall (λ (a:Addr), is_Some (std W !! a)) l →
-     i ∈ dom (std W) ↔ i ∈ dom (std (std_update_multiple W l ρ)).
+   Lemma std_update_multiple_in_sta_i WC (l: list Addr) ρ i :
+     Forall (λ (a:Addr), is_Some (std WC !! a)) l →
+     i ∈ dom (std WC) ↔ i ∈ dom (std (std_update_multiple WC l ρ)).
    Proof.
      intros Hl.
      induction l; auto.
@@ -204,9 +229,9 @@ Section std_updates.
      rewrite elem_of_union elem_of_singleton. intros [-> | Hi]; [| set_solver].
      rewrite elem_of_dom //.
    Qed.
-   Lemma std_update_multiple_not_in_sta W l ρ (a : Addr) :
-     a ∉ l → a ∈ dom (std W) ↔
-             a ∈ dom (std (std_update_multiple W l ρ)).
+   Lemma std_update_multiple_not_in_sta WC l ρ (a : Addr) :
+     a ∉ l → a ∈ dom (std WC) ↔
+             a ∈ dom (std (std_update_multiple WC l ρ)).
    Proof.
      intros Hnin.
      apply std_update_multiple_not_in_sta_i.
@@ -216,27 +241,41 @@ Section std_updates.
    (* ---------------------------------------------------------------------------- *)
    (* Some helper lemmas for various lemmas about using multiple updates in region *)
 
-   Lemma related_sts_pub_update_multiple W l ρ :
-     Forall (λ a, a ∉ dom (std W)) l →
-     related_sts_pub_world W (std_update_multiple W l ρ).
+   Lemma related_sts_pub_update_multiple_cview WC l ρ :
+     Forall (λ a, a ∉ dom (std WC)) l →
+     related_sts_pub_cview WC (std_update_multiple WC l ρ).
    Proof.
      intros Hforall. induction l.
-     - apply related_sts_pub_refl_world.
+     - apply related_sts_pub_refl_cview.
      - simpl.
        apply list.Forall_cons in Hforall as [ Ha_std Hforall].
-       eapply related_sts_pub_trans_world;[apply IHl; auto|].
+       eapply related_sts_pub_trans_cview;[apply IHl; auto|].
        destruct (decide (a ∈ l)).
-       { rewrite (_: <s[a:=ρ]s>(std_update_multiple W l ρ) = std_update_multiple W l ρ) /=.
-         by apply related_sts_pub_refl_world.
-         rewrite /std_update insert_id /=. by destruct (std_update_multiple W l ρ).
+       { rewrite (_: <s[a:=ρ]s>(std_update_multiple WC l ρ) = std_update_multiple WC l ρ) /=.
+         by apply related_sts_pub_refl_cview.
+         rewrite /std_update insert_id /=. by destruct (std_update_multiple WC l ρ).
          by apply std_sta_update_multiple_lookup_in_i. }
-       apply related_sts_pub_world_fresh; auto.
+       apply related_sts_pub_cview_fresh; auto.
        intros Hcontr. apply std_update_multiple_not_in_sta in Hcontr; auto.
    Qed.
 
-   Lemma std_update_multiple_lookup W l ρ k y :
+   Lemma related_sts_pub_update_multiple W C l ρ :
+     Forall (λ a, a ∉ dom (std_C W C)) l →
+     related_sts_pub_world W (std_update_multiple_C W C l ρ) C.
+   Proof.
+     intros Hforall.
+     rewrite /std_C in Hforall.
+     rewrite /std_update_multiple_C.
+     destruct (W!!C) as [WC|] eqn:HWC;last apply related_sts_pub_refl_world.
+     split.
+     - rewrite dom_insert_L ; set_solver.
+     - intros ? WC' ? HWC' ; rewrite lookup_insert in HWC' ; simplify_eq.
+       by apply related_sts_pub_update_multiple_cview.
+   Qed.
+
+   Lemma std_update_multiple_lookup_cview WC l ρ k y :
      l !! k = Some y ->
-     std (std_update_multiple W l ρ) !! y = Some ρ.
+     std (std_update_multiple WC l ρ) !! y = Some ρ.
    Proof.
      intros Helem.
      apply elem_of_list_lookup_2 in Helem.
@@ -245,18 +284,31 @@ Section std_updates.
      rewrite /std /=. rewrite lookup_insert. auto.
    Qed.
 
-   Lemma std_update_temp_multiple_lookup W l k y :
-     l !! k = Some y →
-     region_state_pwl (std_update_temp_multiple W l) y.
+   Lemma std_update_multiple_lookup W C l ρ k y :
+     l !! k = Some y ->
+     is_Some (W!!C) ->
+     std_C (std_update_multiple_C W C l ρ) C !! y = Some ρ.
    Proof.
-     apply std_update_multiple_lookup.
+     intros Helem [WC HWC].
+     rewrite /std_C /std_update_multiple_C HWC.
+     rewrite lookup_insert. eapply std_update_multiple_lookup_cview; eauto.
+   Qed.
+
+   Lemma std_update_temp_multiple_lookup W C l k y :
+     l !! k = Some y →
+     is_Some (W!!C) ->
+     region_state_pwl (std_update_temp_multiple_C W C l) C y.
+   Proof.
+     intros Helem HWC.
+     rewrite /std_update_temp_multiple_C.
+     eapply std_update_multiple_lookup; eauto.
    Qed.
 
 
    (* Multiple updates does not change dom, as long as the updated elements are a subset of original dom *)
-   Lemma std_update_multiple_dom_equal W l ρ :
-     (∀ i : Addr, i ∈ l → i ∈ dom (std W)) ->
-     dom (std W) = dom (std (std_update_multiple W l ρ)).
+   Lemma std_update_multiple_dom_equal WC l ρ :
+     (∀ i : Addr, i ∈ l → i ∈ dom (std WC)) ->
+     dom (std WC) = dom (std (std_update_multiple WC l ρ)).
    Proof.
      intros Hsub.
      induction l; auto.
@@ -270,8 +322,8 @@ Section std_updates.
    Qed.
 
    (* In general, the domain is a subset of the updated domain *)
-   Lemma std_update_multiple_sta_dom_subseteq W l ρ :
-     dom (std W) ⊆ dom (std (std_update_multiple W l ρ)).
+   Lemma std_update_multiple_sta_dom_subseteq WC l ρ :
+     dom (std WC) ⊆ dom (std (std_update_multiple WC l ρ)).
    Proof.
      apply elem_of_subseteq. intros x Hx.
      destruct (decide (x ∈ l)).
@@ -280,26 +332,47 @@ Section std_updates.
      - apply std_update_multiple_not_in_sta_i; auto.
    Qed.
 
-   Lemma std_update_multiple_std_sta_dom_monotone W W' l ρ :
-     dom (std W) ⊆ dom (std W') ->
-     dom (std (std_update_multiple W l ρ)) ⊆ dom (std (std_update_multiple W' l ρ)).
+   Lemma std_update_multiple_std_sta_dom_monotone_cview WC WC' l ρ :
+     dom (std WC) ⊆ dom (std WC') ->
+     dom (std (std_update_multiple WC l ρ)) ⊆ dom (std (std_update_multiple WC' l ρ)).
    Proof.
      induction l;auto.
      simpl. repeat rewrite dom_insert_L. set_solver.
    Qed.
 
-   Lemma std_update_mutiple_related_monotone W W' l ρ :
-     related_sts_pub_world W W' ->
-     related_sts_pub_world (std_update_multiple W l ρ) (std_update_multiple W' l ρ).
+   Lemma std_update_multiple_std_sta_dom_monotone W W' C l ρ :
+     dom W ⊆ dom W' ->
+     dom (std_C W C) ⊆ dom (std_C W' C) ->
+     dom (std_C (std_update_multiple_C W C l ρ) C) ⊆ dom (std_C (std_update_multiple_C W' C l ρ) C).
+   Proof.
+     rewrite /std_C /std_update_multiple_C.
+     intros Hdom_W Hdom.
+     destruct (W !! C) as [WC|] eqn:HWC; last rewrite HWC; eauto; cycle 1.
+     - rewrite dom_empty_L; set_solver.
+     - rewrite lookup_insert.
+       assert (is_Some (W' !! C)) as [WC' HWC'].
+       {
+         apply (elem_of_dom_2 W) in HWC.
+         specialize (Hdom_W _ HWC).
+         by eapply (elem_of_dom W').
+       }
+       rewrite HWC' lookup_insert.
+       rewrite HWC' in Hdom.
+       by eapply std_update_multiple_std_sta_dom_monotone_cview.
+   Qed.
+
+   Lemma std_update_mutiple_related_monotone_cview WC WC' l ρ :
+     related_sts_pub_cview WC WC' ->
+     related_sts_pub_cview (std_update_multiple WC l ρ) (std_update_multiple WC' l ρ).
    Proof.
      intros Hrelated.
-     destruct W as [ Wstd_sta [Wloc_sta Wloc_rel] ].
-     destruct W' as [ Wstd_sta' [Wloc_sta' Wloc_rel'] ].
+     destruct WC as [ Wstd_sta [Wloc_sta Wloc_rel] ].
+     destruct WC' as [ Wstd_sta' [Wloc_sta' Wloc_rel'] ].
      destruct Hrelated as [ [Hstd_dom1 Hstd_related ] Hloc_related].
      simpl in *.
      split;[clear Hloc_related|by repeat rewrite std_update_multiple_loc_rel std_update_multiple_loc_sta].
      split.
-     - apply std_update_multiple_std_sta_dom_monotone. auto.
+     - apply std_update_multiple_std_sta_dom_monotone_cview. auto.
      - intros i x y Hx Hy.
        destruct (decide (i ∈ l)).
        + rewrite std_sta_update_multiple_lookup_in_i in Hx;auto.
@@ -310,6 +383,44 @@ Section std_updates.
          apply Hstd_related with i; auto.
    Qed.
 
+   Lemma std_update_mutiple_dom_monotone W W' C l ρ :
+     dom W ⊆ dom W' ->
+     dom (std_update_multiple_C W C l ρ) ⊆ dom (std_update_multiple_C W' C l ρ).
+    Proof.
+      intros Hdom.
+      rewrite /std_update_multiple_C.
+      destruct (W !! C) as [WC|] eqn:HWC; eauto.
+      - destruct (W' !! C) as [WC'|] eqn:HWC'; eauto.
+        + rewrite !dom_insert_L; set_solver.
+        + eapply (elem_of_dom_2 W) in HWC.
+          specialize (Hdom _ HWC).
+          by eapply (not_elem_of_dom W') in HWC'.
+      - destruct (W' !! C) as [WC'|] eqn:HWC'; eauto.
+        rewrite !dom_insert_L; set_solver.
+    Qed.
+
+   Lemma std_update_mutiple_related_monotone W W' C l ρ :
+     related_sts_pub_world W W' C ->
+     related_sts_pub_world (std_update_multiple_C W C l ρ) (std_update_multiple_C W' C l ρ) C.
+   Proof.
+     intros [Hdom Hrelated].
+     split.
+     - by apply std_update_mutiple_dom_monotone.
+     - rewrite /std_update_multiple_C.
+       intros WC_upd WC_upd' HWC_upd HWC_upd'.
+       destruct (W!!C) as [WC|] eqn:HWC.
+       + destruct (W'!!C) as [WC'|] eqn:HWC' ; cycle 1.
+         { eapply (elem_of_dom_2 W) in HWC.
+           specialize (Hdom _ HWC).
+           by eapply (not_elem_of_dom W') in HWC'.
+         }
+         rewrite lookup_insert in HWC_upd; rewrite lookup_insert in HWC_upd'; simplify_eq.
+         apply std_update_mutiple_related_monotone_cview.
+         by apply Hrelated.
+       + destruct (W'!!C) as [WC'|] eqn:HWC'; simplify_eq.
+   Qed.
+
+   (* TODO update from here if necessary only *)
    (* lemmas for updating a repetition of top *)
    Lemma std_update_multiple_dom_top_sta W n ρ a :
      a ≠ addr_reg.top ->
